Remove all cheats from loo_call pass

pancake/proofs/loop_callProofScript.sml
@@ -8,15 +8,16 @@ open preamble
 
 val _ = new_theory "loop_callProof";
 
+Definition labels_in_def:
+  labels_in l locals =
+    !n x. lookup n l = SOME x ==> lookup n locals = SOME (Loc x 0)
+End
+
 val goal =
   “λ(prog, s). ∀res s1 l p nl.
     evaluate (prog,s) = (res,s1) ∧ res ≠ SOME Error ∧
-    comp l prog = (p, nl) /\
-    (∀n x. lookup n l = SOME x ==> lookup n s.locals = SOME (Loc x 0)) ==>
-    evaluate (p,s) = (res,s1) /\
-    case res of
-     | NONE => (∀n x. lookup n nl = SOME x ==> lookup n s1.locals = SOME (Loc x 0))
-     | _ => T ”
+    comp l prog = (p, nl) /\ labels_in l s.locals ==>
+    evaluate (p,s) = (res,s1) /\ labels_in nl s1.locals”
 
 local
   val ind_thm = loopSemTheory.evaluate_ind |> ISPEC goal
@@ -34,11 +35,9 @@ end
 Theorem compile_Seq:
   ^(get_goal "comp _ (loopLang$Seq _ _)")
 Proof
-  rpt gen_tac >>
-  strip_tac >>
-  rpt gen_tac >>
-  strip_tac >>
-  fs [loopSemTheory.evaluate_def] >>
+  rpt gen_tac >> strip_tac >>
+  rpt gen_tac >> strip_tac >>
+  fs [loopSemTheory.evaluate_def, labels_in_def] >>
   pairarg_tac >> fs [comp_def] >>
   rpt (pairarg_tac >> fs []) >>
   fs [evaluate_def] >>
@@ -55,13 +54,12 @@ Proof
    CCONTR_TAC >> fs []) >>
   strip_tac >> rveq >>
   fs [evaluate_def] >> rveq >> fs [] >>
-  last_x_assum (qspecl_then [‘nl'’, ‘nq’, ‘nl’] mp_tac) >>
-  fs []) >>
+  last_x_assum (qspecl_then [‘nl'’, ‘nq’, ‘nl''’] mp_tac) >>
+  fs [lookup_def]) >>
   first_x_assum (qspecl_then [‘l’, ‘np’, ‘nl'’] mp_tac) >>
   fs [] >>
   strip_tac >>
-  fs [evaluate_def] >> rveq >> fs [] >>
-  cases_on ‘res’ >> fs []
+  fs [evaluate_def, lookup_def]
 QED
 
 
@@ -70,7 +68,7 @@ Theorem compile_LocValue:
 Proof
   rpt gen_tac >>
   strip_tac >>
-  fs [evaluate_def, comp_def] >>
+  fs [evaluate_def, labels_in_def, comp_def] >>
   rveq >> fs [] >>
   fs [evaluate_def] >>
   cases_on ‘res’ >> fs []  >>
@@ -87,7 +85,7 @@ Theorem compile_Assign:
 Proof
   rpt gen_tac >>
   strip_tac >>
-  fs [evaluate_def, comp_def] >>
+  fs [evaluate_def, labels_in_def, comp_def] >>
   rveq >> fs [] >>
   fs [evaluate_def] >>
   cases_on ‘res’ >> fs []  >>
@@ -105,7 +103,7 @@ Theorem compile_LoadByte:
 Proof
   rpt gen_tac >>
   strip_tac >>
-  fs [evaluate_def, comp_def] >>
+  fs [evaluate_def,labels_in_def, comp_def] >>
   rveq >> fs [] >>
   fs [evaluate_def] >>
   cases_on ‘res’ >> fs []  >>
@@ -141,7 +139,7 @@ Proof
   rpt gen_tac >>
   strip_tac >>
   rpt gen_tac >>
-  fs [comp_def] >>
+  fs [labels_in_def, comp_def] >>
   every_case_tac >> fs [] >>
   rveq >> fs [] >>
   fs [evaluate_def] >>
@@ -158,7 +156,7 @@ Proof
   strip_tac >>
   rpt gen_tac >>
   strip_tac >>
-  fs [evaluate_def, comp_def] >>
+  fs [evaluate_def, labels_in_def, comp_def] >>
   rveq >> fs [] >>
   fs [evaluate_def, CaseEq "option", CaseEq "word_loc"] >>
   rveq >> fs [] >>
@@ -174,25 +172,15 @@ Proof
     fs [] >>
     strip_tac >> fs [] >>
     fs [evaluate_def] >>
-    cases_on ‘q’ >> fs [cut_res_def]) >>
+    cases_on ‘q’ >> fs [cut_res_def, lookup_def]) >>
    last_x_assum drule >>
    fs [] >>
    strip_tac >> fs [CaseEq "option"] >>
    rveq >> fs []  >>
-   fs [evaluate_def] >>
-   fs [cut_res_def] >>
-   cases_on ‘v.clock = 0’ >> fs [] >> rveq >> fs [] >>
-   fs [dec_clock_def, lookup_inter, cut_state_def] >>
-   qpat_x_assum ‘r with locals := _ = _’ (assume_tac o GSYM) >>
-   rveq >> fs [] >>
-   rw [] >>
-   fs [CaseEq "option"] >> rveq >> fs [lookup_inter] >>
-   res_tac >>
-   TOP_CASE_TAC >> fs [] >> rveq >>
-   fs [lookup_def] >>
-   TOP_CASE_TAC >> fs []) >>
+   fs [evaluate_def, lookup_def] >>
+   fs [cut_res_def]) >>
   cases_on ‘evaluate (c2,s)’ >> fs [] >>
-  fs [cut_res_def] >>
+  fs [cut_res_def, lookup_def] >>
   cases_on ‘q ≠ NONE’ >> fs [] >> rveq >> fs []
   >- (
    last_x_assum drule >>
@@ -205,17 +193,7 @@ Proof
   strip_tac >> fs [CaseEq "option"] >>
   rveq >> fs []  >>
   fs [evaluate_def] >>
-  fs [cut_res_def] >>
-  cases_on ‘v.clock = 0’ >> fs [] >> rveq >> fs [] >>
-  fs [dec_clock_def, lookup_inter, cut_state_def] >>
-  qpat_x_assum ‘r with locals := _ = _’ (assume_tac o GSYM) >>
-  rveq >> fs [] >>
-  rw [] >>
-  fs [CaseEq "option"] >> rveq >> fs [lookup_inter] >>
-  res_tac >>
-  TOP_CASE_TAC >> fs [] >> rveq >>
-  fs [lookup_def] >>
-  TOP_CASE_TAC >> fs []
+  fs [cut_res_def]
 QED
 
 Theorem compile_StoreByte:
@@ -223,7 +201,7 @@ Theorem compile_StoreByte:
 Proof
   rpt gen_tac >>
   strip_tac >>
-  fs [evaluate_def, comp_def] >>
+  fs [evaluate_def, labels_in_def, comp_def] >>
   rveq >> fs [] >>
   fs [evaluate_def] >>
   cases_on ‘res’ >> fs []  >>
@@ -238,127 +216,13 @@ Theorem compile_Store:
 Proof
   rpt gen_tac >>
   strip_tac >>
-  fs [evaluate_def, comp_def] >>
+  fs [evaluate_def, labels_in_def, comp_def] >>
   rveq >> fs [] >>
   fs [evaluate_def] >>
   cases_on ‘res’ >> fs []  >>
   every_case_tac >> fs [mem_store_def] >>
   last_x_assum (assume_tac o GSYM) >>
   rveq >> fs []
-QED
-
-
-Theorem compile_Call:
-  ^(get_goal "comp _ (loopLang$Call _ _ _ _)")
-Proof
-  cheat
-QED
-
-Theorem compile_Loop:
-  ^(get_goal "comp _ (loopLang$Loop _ _ _)")
-Proof
-  rpt gen_tac >>
-  strip_tac >>
-  rpt gen_tac >>
-  strip_tac >>
-  fs [Once evaluate_def, comp_def] >>
-  cases_on ‘cut_res live_in (NONE:'a result option,s)’ >> fs [] >>
-  rveq >> fs [] >>
-  pairarg_tac >>
-  fs [] >>
-  reverse (cases_on ‘q’) >> fs [] >> rveq >> fs []
-  >- fs [Once evaluate_def] >>
-  cases_on ‘evaluate (body,r)’ >> fs [] >>
-  cases_on ‘q’ >> fs [] >>
-  cases_on ‘x’ >> fs [] >>
-  rveq >> fs [] >>
-  fs [Once evaluate_def] >>
-  res_tac >> fs [] >>
-  cheat
-QED
-
-
-Theorem compile_others:
-  ^(get_goal "comp _ loopLang$Skip") ∧
-  ^(get_goal "comp _ loopLang$Fail") ∧
-  ^(get_goal "comp _ loopLang$Tick") ∧
-  ^(get_goal "comp _ loopLang$Break") ∧
-  ^(get_goal "comp _ loopLang$Continue") ∧
-  ^(get_goal "comp _ (loopLang$Raise _)") ∧
-  ^(get_goal "comp _ (loopLang$Return _)") ∧
-  ^(get_goal "comp _ (loopLang$SetGlobal _ _)")
-Proof
-  rw [] >>
-  fs [evaluate_def, comp_def] >>
-  rveq >> fs [] >>
-  fs [evaluate_def] >>
-  cases_on ‘res’ >>
-  fs [] >>
-  every_case_tac >> fs [dec_clock_def] >>
-  last_x_assum (assume_tac o GSYM) >>
-  rveq >> fs [set_globals_def]
-QED
-
-
-Theorem compile_correct:
-  ^(compile_correct_tm())
-Proof
-  match_mp_tac (the_ind_thm()) >>
-  EVERY (map strip_assume_tac
-         [compile_others,compile_LocValue,compile_LoadByte,compile_StoreByte,
-          compile_Mark, compile_Assign, compile_Store,
-          compile_Call, compile_Seq, compile_If, compile_FFI, compile_Loop]) >>
-  asm_rewrite_tac [] >> rw [] >> rpt (pop_assum kall_tac)
-QED
-
-
-
-
-(*
-(*
-Theorem butlast_cons:
-  !xs x. xs <> [] ==>
-    butlast (x::xs) = x::butlast xs
-Proof
-  Induct >>
-  rw [] >>
-  fs [butlast_def]
-QED
-
-
-Theorem last_cons:
-  !xs x. xs <> [] ==>
-    last (x::xs) = LAST xs
-Proof
-  Induct >>
-  rw [] >>
-  fs [last_def] >>
-  cases_on ‘xs’ >>
-  fs [LAST_DEF, EL]
-QED
-
-Theorem butlast_front_eq:
-  !xs. xs <> [] ==>
-  butlast xs = FRONT xs
-Proof
-  Induct >>
-  rw [] >>
-  fs [FRONT_DEF] >>
-  every_case_tac >> fs []
-  >- fs [butlast_def] >>
-  metis_tac [butlast_cons]
-QED
-
-Theorem last_last_eq:
-  !xs. xs <> [] ==>
-  last xs = LAST xs
-Proof
-  Induct >>
-  rw [] >>
-  fs [LAST_DEF] >>
-  every_case_tac >> fs []
-  >- fs [last_def] >>
-  metis_tac [last_cons]
 QED
 
 Theorem get_vars_front:
@@ -387,6 +251,7 @@ Proof
   every_case_tac >> fs []
 QED
 
+
 Theorem get_vars_last:
   !xs ys s. get_vars xs s = SOME ys /\ xs <> []==>
    lookup (LAST xs) s.locals = SOME (LAST ys)
@@ -412,131 +277,42 @@ Proof
   fs [get_vars_def] >>
   every_case_tac >> fs []
 QED
-*)
 
-Theorem comp_correct:
-  !prog s res s1 l. loopSem$evaluate (prog,s) = (res,s1) ∧
-  res ≠ SOME Error ∧
-  (∀n x. lookup n l = SOME x ==> lookup n s.locals = SOME (Loc x 0)) /\
-  comp l prog = (np, nl) /\ evaluate (np,s) = (res',s1') ==>
-   (res = res' /\ s1 = s1' /\
-    (∀n x. lookup n nl = SOME x ==> lookup n s1.locals = SOME (Loc x 0)))
+Theorem compile_Call:
+  ^(get_goal "comp _ (loopLang$Call _ _ _ _)")
 Proof
-  ho_match_mp_tac loopSemTheory.evaluate_ind >>
-
-
-
-  cases_on ‘prog’ >>
-  fs [loop_callTheory.comp_def]
-  >- (fs [evaluate_def] >> rveq >> fs [])
+  rpt gen_tac >>
+  strip_tac >>
+  rpt gen_tac >>
+  rpt (pop_assum kall_tac) >>
+  strip_tac >>
+  reverse (cases_on ‘dest’)
   >- (
-   fs [evaluate_def] >>
-   every_case_tac >> fs [] >> rveq  >> fs [] >>
-   rw []
-   >- (
-    fs [set_var_def] >>
-    fs [lookup_insert] >>
-    TOP_CASE_TAC >> fs []) >>
-   fs [set_var_def] >>
-   fs [lookup_insert] >>
-   TOP_CASE_TAC >> fs [] >> rveq >>
-   fs [lookup_delete])
-  >- (
-   fs [evaluate_def] >>
-   every_case_tac >> fs [] >> rveq  >> fs [] >>
-   rw [] >>
-   fs [mem_store_def] >>
-   pop_assum mp_tac >>
-   pop_assum (assume_tac o GSYM) >>
-   fs [])
-  >- (
-   fs [evaluate_def] >>
-   every_case_tac >> fs [] >> rveq  >> fs [] >>
-   rw [] >>
-   fs [set_globals_def])
-  >- (
-   fs [evaluate_def] >>
-   every_case_tac >> fs [] >> rveq  >> fs [] >>
-   rw [] >>
-   fs [set_var_def, lookup_insert] >>
-   TOP_CASE_TAC >> fs [] >>
-   rveq >> fs [lookup_delete])
-  >- (
-   fs [evaluate_def] >>
-   every_case_tac >> fs [] >> rveq  >> fs [])
-
-
-
-  >- (
-   fs [evaluate_def] >>
-   pairarg_tac >> fs [] >>
+   fs [loop_callTheory.comp_def] >>
    rveq >> fs [] >>
-   cases_on ‘res' = NONE’ >> fs [] >>
-   rveq >> fs []
-
-
-   pairarg_tac >> fs [] >>
-   pairarg_tac >> fs [] >>
-   pairarg_tac >> fs [] >> rveq >>
-   every_case_tac >> fs [] >> rveq  >> fs [] >>
-   pairarg_tac >> fs [] >> rveq >>
-   pairarg_tac >> fs [] >> rveq >>
-   every_case_tac >> fs [] >>
-
-
-   )
-
-   )
-
-
-
-
-   )
-
-
-
-
-
-
-   )
-
-
-
-   )
-
-    )
-
-      rveq >> fs [])
-
-
-
-
-  qmatch_goalsub_rename_tac ‘Call ret dest args hdl’ >>
-  cases_on ‘dest’ >>
-  fs [loop_callTheory.comp_def] >>
-  ‘args <> []’ by (
-    CCONTR_TAC >> fs [] >> rveq >>
-    fs [evaluate_def, get_vars_def, find_code_def]) >>
-  fs [] >>
-  TOP_CASE_TAC >> fs [] >>
+   fs [labels_in_def, lookup_def]) >>
+  cases_on ‘argvars’
+  >- (
+   fs [loop_callTheory.comp_def, evaluate_def, get_vars_def] >>
+   fs [find_code_def]) >>
+  fs [loop_callTheory.comp_def] >> rveq >>
+  TOP_CASE_TAC >> fs []
+  >- fs [labels_in_def, lookup_def] >>
+  fs [labels_in_def, lookup_def] >>
   fs [evaluate_def] >>
-  cases_on ‘get_vars args s’ >> fs [] >>
-  qmatch_asmsub_rename_tac ‘get_vars args _ = SOME argsval’ >>
+  cases_on ‘get_vars (h::t) s’ >> fs [] >>
+  qmatch_asmsub_rename_tac ‘get_vars (h::t) _ = SOME argsval’ >>
   cases_on ‘find_code NONE argsval s.code’ >>
   fs [] >>
-  ‘get_vars (butlast args) s = SOME (FRONT argsval)’ by (
+  ‘get_vars (FRONT (h::t)) s = SOME (FRONT argsval)’ by (
     fs [] >>
-    drule butlast_front_eq >>
-    fs [] >>
-    strip_tac >>
-    metis_tac [get_vars_front]) >>
+    drule get_vars_front >>
+    fs []) >>
   fs [] >>
   ‘find_code (SOME x) (FRONT argsval) s.code = SOME x'’ suffices_by fs [] >>
   ‘LAST argsval = (Loc x 0)’ by (
-    ‘LAST argsval = THE(lookup (last args) s.locals)’ by (
-      ‘last args = LAST args’ by metis_tac [last_last_eq] >>
+    ‘LAST argsval = THE(lookup (LAST (h::t)) s.locals)’ by (
       fs [] >>
-      pop_assum mp_tac >>
       pop_assum mp_tac >>
       drule get_vars_last >>
       fs []) >>
@@ -547,6 +323,64 @@ Proof
   TOP_CASE_TAC >> fs [] >>
   fs [LENGTH_FRONT]
 QED
-*)
+
+
+Theorem compile_Loop:
+  ^(get_goal "comp _ (loopLang$Loop _ _ _)")
+Proof
+  rpt gen_tac >> strip_tac >>
+  rpt gen_tac >> strip_tac >>
+  fs [comp_def] >>
+  pairarg_tac >> fs [] >>
+  rveq >> fs [] >>
+  qpat_x_assum ‘evaluate (Loop _ _ _,_) = (_,_)’ mp_tac >>
+  once_rewrite_tac [evaluate_def] >>
+  TOP_CASE_TAC >> fs [] >> rveq >>
+  reverse TOP_CASE_TAC >> fs [] >> rveq >> fs []
+  >- (
+   strip_tac >> rveq >>
+   fs [labels_in_def, lookup_def]) >>
+  TOP_CASE_TAC >> fs [] >> rveq >> fs [] >>
+  TOP_CASE_TAC >> fs [] >> rveq >> fs [] >>
+  TOP_CASE_TAC >> fs [] >> rveq >> fs [] >> (
+  strip_tac >> rveq >> fs [] >>
+  res_tac >> fs [labels_in_def, lookup_def]) >>
+  first_x_assum (qspec_then ‘LN’ mp_tac) >>
+  fs [labels_in_def, lookup_def]
+QED
+
+
+Theorem compile_others:
+  ^(get_goal "comp _ loopLang$Skip") ∧
+  ^(get_goal "comp _ loopLang$Fail") ∧
+  ^(get_goal "comp _ (loopLang$SetGlobal _ _)") ∧
+  ^(get_goal "comp _ loopLang$Tick") ∧
+  ^(get_goal "comp _ loopLang$Break") ∧
+  ^(get_goal "comp _ loopLang$Continue") ∧
+  ^(get_goal "comp _ (loopLang$Return _)") ∧
+  ^(get_goal "comp _ (loopLang$Raise _)")
+Proof
+  rpt conj_tac >>
+  rpt gen_tac >> strip_tac >>
+  fs [evaluate_def, labels_in_def, comp_def] >>
+  rveq >> fs [] >>
+  fs [evaluate_def] >>
+  every_case_tac >> fs [dec_clock_def] >>
+  last_x_assum (assume_tac o GSYM) >>
+  rveq >> fs [set_globals_def, lookup_def]
+QED
+
+
+Theorem compile_correct:
+  ^(compile_correct_tm())
+Proof
+  match_mp_tac (the_ind_thm()) >>
+  EVERY (map strip_assume_tac
+         [compile_others,compile_LocValue,compile_LoadByte,compile_StoreByte,
+          compile_Mark, compile_Assign, compile_Store,
+          compile_Call, compile_Seq, compile_If, compile_FFI, compile_Loop]) >>
+  asm_rewrite_tac [] >> rw [] >> rpt (pop_assum kall_tac)
+QED
+
 
 val _ = export_theory();
